lib/BisimChecker.v
@@ -115,6 +115,9 @@ Section BisimChecker.
   Proof.
   Admitted.
 
+  Definition state_temp_prod_eqdec : forall (x y: state_template a * state_template a), {x = y} + {x <> y} :=
+    fun x y => EquivDec.prod_eqdec _ _ x y. 
+
 End BisimChecker.
 
 Lemma forall_exists:
@@ -381,6 +384,30 @@ Ltac print_rel_len :=
   clear foo;
   clear bar.
 
+
+  Fixpoint in_checker {A} (A_eq: forall (x y: A), ({x = y} + {x <> y})%type) (x: A) (xs : list A) : bool :=
+    match xs with
+    | nil => false
+    | x' :: xs' => 
+      if A_eq x' x then true else in_checker A_eq x xs'
+    end.
+  
+  Lemma in_checker_conv : 
+    forall A A_eq x xs, 
+      (@in_checker A A_eq x xs = true) -> List.In x xs.
+  Proof.
+    intros.
+    induction xs; [inversion H|].
+    
+    simpl in_checker in H.
+    destruct (A_eq _ _).
+    - econstructor; assumption.
+    - eapply or_intror.
+      eapply IHxs.
+      assumption.
+  Qed. 
+
+
 Ltac close_bisim top' :=
   apply PreBisimulationClose;
   match goal with
@@ -410,6 +437,43 @@ Ltac close_bisim top' :=
            end;
     subst;
     simpl; tauto
+  end.
+
+Ltac close_bisim' top' := 
+  eapply PreBisimulationClose;
+  match goal with
+  | H: interp_conf_rel' ?C ?q1 ?q2|- interp_crel _ ?top ?P ?q1 ?q2 =>
+    let H0 := fresh "H0" in
+    assert (H0: interp_entailment' top {| e_prem := P; e_concl := C |}) by (
+      eapply simplify_entailment_correct' with (i := top');
+      eapply compile_simplified_entailment_correct';
+
+      simpl; intros;
+      eapply FirstOrderConfRelSimplified.simplify_eq_zero_fm_corr;
+      eapply CompileFirstOrderConfRelSimplified.compile_simplified_fm_bv_correct;
+
+      crunch_foterm;
+      match goal with
+      | |- ?X => time "smt check pos" check_interp_pos X; admit
+      end
+    );
+    eapply H0; 
+    destruct q1, q2;
+    vm_compute in H;
+    repeat match goal with 
+    | H: _ /\ _ |- _ => destruct H
+    end;
+    [
+      apply in_checker_conv with (A_eq := fun x y => state_temp_prod_eqdec x y);
+      unfold conf_to_state_template, P4automaton.conf_buf_len, P4automaton.conf_state;
+    
+      repeat match goal with 
+      | H: _ = _ |- _ => erewrite <- H
+      end;
+      exact eq_refl
+                    |
+      split; [ vm_compute; (repeat split || assumption) | (intros; exact I)]
+    ]
   end.
 
 (* solves a header finiteness goal of the form:
